src/Concurrent/Bisim.v
@@ -1,14 +1,26 @@
 
 (*
-  Things to think about:
-  - PID-compatibility - bijectivity between the refered and taken PIDs in a system
-    - (refered PIDs -- taken PIDs) <- does this give the context?
-  - Does db-indexing PIDs make sense?
-  -
-
+  Lessons learned:
+  - PIDsOf cannot be defined for the co-inductive version
+  - using functions for process pools is
+    - simple for the definitions
+    - hard, if its properties (e.g., dom) is needed
+  - Bisimulations
+    - Playing with bisimulation in Erlang -> this paper only considers ethers
+      and defines observations based on the "dangling" messages
+    - The usual notion of bisimulations involves checking equality on actions, 
+      however, in this case we could not reason about systems using different 
+      PIDs.
+    - Bisimulations + bijective function on the PIDs? Drawback: we have to 
+      somehow rename all PIDs in signals/messages, which might be impossible
+      for closure values (because they include a body expression which could
+      contain e.g., "self()" calls, where the PID is not syntactically there).
+        ^---- would be enough to observe the "type" of these actions?
+      - How "deep" action parameters should be investigated? Should they
+        be equivalent, or check only the type, or nothing?
 *)
 
-From CoreErlang Require Import Concurrent.NodeSemantics.
+From CoreErlang Require Import Concurrent.InductiveNodeSemantics.
 
 Import ListNotations.
 
@@ -24,7 +36,33 @@ Definition isPreCompatible (Π₁ Π₂ : ProcessPool) : Prop :=
 
 (* Definition isCompatible (Π₁ Π₂ : ProcessPool) : Prop :=
   isPreCompatible Π₁ Π₂ /\ isPreCompatible Π₂ Π₁. *)
+Goal
+  isPreCompatible
+    (0 ↦ inl ([], RExp (`VNil), ([], []), [], false) |||| 1 ↦ inl ([], RExp (`VNil), ([], []), [], false) |||| nullpool)
+    (0 ↦ inl ([], RExp (`VNil), ([], []), [], false) |||| 1 ↦ inr [] |||| nullpool).
+Proof.
+  unfold isPreCompatible, isUnTaken in *.
+  intros.
+  destruct ι; cbn in *.
+  congruence.
+  destruct ι; cbn in *.
+  congruence.
+  assumption.
+Qed.
 
+Goal
+  isPreCompatible
+    (10 ↦ inl ([], RExp (`VNil), ([], []), [], false) |||| 13 ↦ inl ([], RExp (`VNil), ([], []), [], false) |||| nullpool)
+    (13 ↦ inl ([], RExp (`VNil), ([], []), [], false) |||| 10 ↦ inr [] |||| nullpool).
+Proof.
+  unfold isPreCompatible, isUnTaken in *.
+  intros.
+  destruct (Nat.eq_dec ι 13).
+  * subst. cbn in *. congruence.
+  * destruct (Nat.eq_dec ι 10).
+    - subst. cbn in *. congruence.
+    - rewrite update_next. rewrite update_next. all: auto.
+Qed.
 
 (** This is needed to ensure that a process is not spawned with a wrong PID
     in the equivalence. *)
@@ -59,7 +97,10 @@ Definition isPreCompatibleReductions
   isPreCompatibleReductions red1 red2 /\
   isPreCompatibleReductions red2 red1. *)
 
-(* This does not say anything about the equivalence of actions *)
+(* This does not say anything about the equivalence of actions
+   TODO: this definition does not include the equivalence of ethers, which
+   is included in Lanese et al. Playing with bisimulation in Erlang
+*)
 Definition simulates (S : Node -> Node -> Prop) :=
   forall n₁ n₁' n₂ a ι (pf : S n₁ n₂) (red : n₁ -[a | ι]ₙ-> n₁'),
     exists n₂' l, n₂ -[l]ₙ->* n₂' /\ isPreCompatibleReductions n₁ n₂ l /\ S n₁' n₂'.
