src/Concurrent/CoNodeSemantics.v
@@ -1,0 +1,24 @@
+From CoreErlang Require Export Concurrent.NodeSemantics.
+From CoreErlang Require Export CoList.
+
+(** Refexive, transitive closure, with action logs: *)
+Reserved Notation "n -[ l ]ₙ->* n'" (at level 50).
+CoInductive closureNodeSem : Node -> Trace (Action * PID) -> Node -> Prop :=
+| n_refl n (* n'  *): (* Permutation n n' -> *) n -[ []ₜ ]ₙ->* n (* ' *)
+| n_trans n n' n'' l a ι:
+  n -[a|ι]ₙ-> n' -> n' -[l]ₙ->* n''
+->
+  n -[(a,ι)::ₜ l]ₙ->* n''
+where "n -[ l ]ₙ->* n'" := (closureNodeSem n l n').
+
+Theorem closureNodeSem_trans :
+  forall n n' l, n -[l]ₙ->* n' -> forall n'' l', n' -[l']ₙ->* n''
+->
+  n -[l ++ₜ l']ₙ->* n''.
+Proof.
+  cofix IHD1; intros n n' l D1; inv D1; intros; simpl.
+  * rewrite trace_append_nil. exact H.
+  * rewrite trace_append_cons.
+    eapply n_trans. exact H.
+    eapply (IHD1 _ _ _ H0) in H1. exact H1.
+Qed.
