src/Concurrent/InductiveNodeSemantics.v
@@ -1,0 +1,25 @@
+From CoreErlang.Concurrent Require Export NodeSemantics.
+
+Import ListNotations.
+
+(** Refexive, transitive closure, with action logs: *)
+Reserved Notation "n -[ l ]ₙ->* n'" (at level 50).
+Inductive closureNodeSem : Node -> list (Action * PID) -> Node -> Prop :=
+| n_refl n (* n'  *): (* Permutation n n' -> *) n -[ [] ]ₙ->* n (* ' *)
+| n_trans n n' n'' l a ι:
+  n -[a|ι]ₙ-> n' -> n' -[l]ₙ->* n''
+->
+  n -[(a,ι)::l]ₙ->* n''
+where "n -[ l ]ₙ->* n'" := (closureNodeSem n l n').
+
+Theorem closureNodeSem_trans :
+  forall n n' l, n -[l]ₙ->* n' -> forall n'' l', n' -[l']ₙ->* n''
+->
+  n -[l ++ l']ₙ->* n''.
+Proof.
+  intros n n' l D1; induction D1; intros; simpl.
+  * exact H.
+  * eapply n_trans. exact H.
+    eapply (IHD1 _ _ H0).
+Qed.
+
